Common/Util.lean
@@ -11,14 +11,59 @@ lemma demorgan : ¬ (A ∨ B) -> ¬ A ∧ ¬ B := by {
   intro h2; apply h (Or.inr h2)
 }
 
-def ne_sym : x ≠ y -> y ≠ x := sorry 
+def ne_sym : x ≠ y -> y ≠ x := by intro h1 h2; subst h2; contradiction
 
-def append_eq {a c : List α} {b d : α} : a ++ [b] = c ++ [d] -> a = c ∧ b = d := sorry
+def append_eq {a c : List α} {b d : α} : a ++ [b] = c ++ [d] -> a = c ∧ b = d := by {
+  intro h
+  induction a generalizing c
+  case nil => {
+    rw [List.nil_append] at h
+    cases c
+    case nil => {
+      rw [List.nil_append] at h
+      injection h with e1 e2; simp [*]
+    }
+    case cons hd tl => injection h with e1 e2; simp at *
+  }
+  case cons hd tl ih => {
+    cases c
+    case nil => injection h with e1 e2; simp at *
+    case cons hd' tl' => {
+      injection h with e1 e2; simp at *
+      have lem := ih e2
+      simp [*]
+    }
+  }
+}
 
-def pair_eq : (a, b) = (c, d) -> a = c ∧ b = d := sorry
+def pair_eq : (a, b) = (c, d) -> a = c ∧ b = d := by {
+  intro h; injection h with e1 e2
+  subst e1; subst e2; simp
+}
 
-def nat_add_le {a b c : Nat} : a + b ≤ c -> a ≤ c ∧ b ≤ c := sorry  
+def fin_cast {i : Nat} : (h : i < i + 1) -> Fin.mk i h = ↑i := by {
+  intro h
+  induction i
+  case zero => simp [*]
+  case succ x ih => {
+    simp; rw [<-Fin.succ_mk _ x, ih (by linarith), Fin.add_def, Fin.succ]; simp
+    have lem1 : (x + 1) ≠ 0 := by linarith
+    have lem2 := (@Nat.mod_eq_iff_lt x _ lem1).2 (by linarith)
+    have lem3 : (Nat.succ x + 1) ≠ 0 := by linarith
+    have lem4 := (@Nat.mod_eq_iff_lt (x + 1) _ lem3).2 (by linarith)
+    rw [lem2, lem4]  
+  }
+}
 
-def fin_cast {i u : Nat} : (h : i < i + 1) -> Fin.mk i h = ↑i := sorry
-
-def fin_cast2 {n : Nat} {i : Fin (n + 1)} : i = ↑i.val := sorry
+def fin_cast2 {n : Nat} {i : Fin (n + 1)} : i = ↑i.val := by {
+  induction i; simp
+  case mk iv il =>
+  induction iv <;> simp
+  case succ x _ih => {
+    have lem : x < n := by linarith
+    rw [<- Fin.succ_mk n x lem, Fin.add_def, Fin.succ]; simp
+    have lem1 : (n + 1) ≠ 0 := by linarith
+    have lem2 := (@Nat.mod_eq_iff_lt (x + 1) _ lem1).2 (by linarith)
+    rw [lem2]
+  }
+}
