Cedille/Lemma.lean
@@ -1,9 +1,11 @@
 
 import Cedille.Lemma.Basic
+import Cedille.Lemma.Classification
 import Cedille.Lemma.Confluence
 import Cedille.Lemma.Conv
 import Cedille.Lemma.Erasure
 import Cedille.Lemma.Inversion
+import Cedille.Lemma.Preservation
 import Cedille.Lemma.Red
 import Cedille.Lemma.RedErasure
 import Cedille.Lemma.Refold
