Cedille/Lemma/Basic.lean
@@ -1,11 +1,12 @@
 
 import Cedille.Def
+import Cedille.Lemma.Refold
 
 namespace Cedille
 
   @[simp] def open_bound_1_0 : {_|-> x}(@bound 1 0) = free x := by {
       unfold HasHOpen.hopn; unfold Syntax.instHasHOpenSyntax; simp
-      unfold Syntax.opn_head; simp; unfold bound; simp; unfold free; simp
+      unfold Syntax.opn_head; simp; unfold bound; simp
   }
 
   @[simp] def open_bound_2_0 : {_|-> x}(@bound 2 0) = @bound 1 0 := by {
@@ -15,7 +16,7 @@ namespace Cedille
 
   @[simp] def open_bound_2_1 : {_|-> x}(@bound 2 1) = free x := by {
     unfold HasHOpen.hopn; unfold Syntax.instHasHOpenSyntax; simp
-    unfold Syntax.opn_head; simp; unfold bound; simp; unfold free; simp
+    unfold Syntax.opn_head; simp; unfold bound; simp
   }
 
   @[simp] lemma fv_id_empty : @fv n (lam mf kindu (bound 0)) = [] := by {
@@ -32,19 +33,16 @@ namespace Cedille
   @[simp] lemma mode_pi_codomain_m0 : Mode.pi_codomain m0 = @typeu n := by congr
   @[simp] lemma mode_pi_codomain_mt : Mode.pi_codomain mt = @kindu n := by congr
 
-  @[simp] lemma mode_lam_domain_mf : Mode.lam_domain mf = @typeu n := by congr
-  @[simp] lemma mode_lam_domain_m0 : Mode.lam_domain m0 = @typeu n := by congr
-  @[simp] lemma mode_lam_domain_mt : Mode.lam_domain mt = @kindu n := by congr
-
-  lemma subset_mem {x : Name} {A B : FvSet!} : A ⊆ B -> x ∈ A -> x ∈ B := sorry
-  @[simp] lemma fv_subst : fv ([_:= t1]t2) = fv t1 ++ fv t2 := sorry
-  @[simp] lemma fv_open : fv ({_|-> x}t) = [x] ++ fv t := sorry
-
-  lemma subset_left {A B C : FvSet!} : A ⊆ B -> A ⊆ B ++ C := sorry
-  lemma subset_right {A B C : FvSet!} : A ⊆ C -> A ⊆ B ++ C := sorry
-  lemma subset_cons {A B : FvSet!} : x ∉ A -> A ⊆ x :: B -> A ⊆ B := sorry
-  lemma subset_trans {A B C : FvSet!} : A ⊆ B -> B ⊆ C -> A ⊆ C := sorry 
-
-  lemma not_mem_subset_not_mem {A B : FvSet!} : x ∉ A -> B ⊆ A -> x ∉ B := sorry
+  @[simp] lemma refl_erased_is_normal : ¬ (lam mf kindu (bound 0) -β> t) := by {
+    intro h
+    cases h
+    case bind1 _ step => cases step
+    case bind2 _ S step => {
+      have xfresh := @Name.fresh_is_fresh S
+      generalize _xdef : Name.fresh S = x at *
+      replace step := step x xfresh
+      simp at *; cases step
+    }
+  }
 
 end Cedille
