Cedille/Lemma/Classification.lean
@@ -1,0 +1,182 @@
+
+import Common
+import Cedille.Def
+import Cedille.Lemma.Basic
+import Cedille.Lemma.Refold
+import Cedille.Lemma.Erasure
+import Cedille.Lemma.Inversion
+import Cedille.Lemma.Red
+
+namespace Cedille
+
+  lemma infer_implies_wf : Γ ⊢ t : A -> ⊢ Γ := sorry
+  lemma cinfer_implies_wf : Γ ⊢ t >: A -> ⊢ Γ := sorry
+
+  lemma project_ctx_proof : ⊢ Γ -> (x, A) ∈ Γ -> ∃ K, Γ ⊢ A >: const K := sorry
+
+  lemma classification_of_check : Γ ⊢ t =: A -> ∃ K, Γ ⊢ A >: const K := by {
+    intro j
+    cases j; case _ A' K j conv j2 =>
+    exists K
+  }
+
+  lemma classification_of_infer : Γ ⊢ t >: A ->
+    A = kindu ∨ ∃ K, Γ ⊢ A >: const K
+  := λ j => @ConInfer.rec
+    (λ Γ t A j => A = kindu ∨ ∃ K, ∀ B, A -β>* B -> Γ ⊢ B >: const K)
+    (λ Γ t A j => A = kindu ∨ ∃ K, Γ ⊢ A >: const K)
+    (λ Γ t A j => A = kindu ∨ ∃ K, Γ ⊢ A >: const K)
+    (λ Γ wf => True)
+  (by {
+    intro Γ wf _
+    apply Or.inl rfl
+  })
+  (by {
+    intro Γ x A wf xn _
+    apply Or.inr _
+    have lem := project_ctx_proof wf xn
+    cases lem; case _ K j =>
+    exists K; intro B step
+    sorry
+  })
+  (by {
+    intro Γ A m K B S j1 j2 ih1 ih2; simp at *
+    cases m <;> simp at *
+    case free => {
+      apply Or.inr _
+      exists Constant.kindU
+      sorry
+    }
+    case erased => {
+      apply Or.inr _
+      exists Constant.kindU
+      sorry
+    }
+  })
+  (by {
+    intro Γ A m K t B S j1 j2 j3 ih1 ih2; simp at *
+    sorry
+  })
+  (by {
+    intro Γ f m A B a S j1 j2 ih1 ih2
+    cases ih1 <;> simp at *
+    case inr h => {
+      casesm* ∃ _, _, _ ∧ _; case _ K A' j step =>
+      sorry
+    }
+  })
+  sorry
+  sorry
+  sorry
+  sorry
+  sorry
+  sorry
+  sorry
+  sorry
+  sorry
+  sorry
+  (by {
+    intro Γ t A B j step ih
+    sorry
+  })
+  (by {
+    intro Γ t A B K j1 j2 conv ih1 ih2
+    apply Or.inr _
+    exists K
+  })
+  (by simp)
+  (by simp)
+  Γ
+  t
+  A
+  j
+
+  lemma classification_of_infer2 : Γ ⊢ t : A ->
+    A = kindu ∨ ∃ K, Γ ⊢ A >: const K
+  := λ j => @Nat.rec
+    (λ s => ∀ Γ t A,
+      size t ≤ s ->
+      Γ ⊢ t >: A ->
+      A = kindu ∨ ∃ K, Γ ⊢ A >: const K)
+    (by {
+      intro Γ t A sh j
+      sorry
+    })
+    (by {
+      intro s ih Γ t A sh j
+      cases t
+      case bound => apply ih Γ (bound _) A (by simp) j
+      case free => apply ih Γ (free _) A (by simp) j
+      case const => apply ih Γ (const _) A (by simp) j
+      case bind b u1 u2 => {
+        simp at *
+        have s1 : size u1 ≤ s := by linarith
+        have s2 : size u2 ≤ s := by linarith
+        cases b <;> simp at *
+        case lam m => {
+          sorry
+        }
+        case pi m => {
+          sorry
+          -- cases j; case _ K S j1 j2 =>
+          -- cases m <;> simp at *
+          -- case free => {
+          --   apply Or.inr; exists Constant.kindU; unfold const; simp
+          --   apply ConInfer.infer _ _; exact kindu
+          --   apply Infer.ax
+          --   apply cinfer_implies_wf j1
+          --   apply RedStar.refl
+          -- }
+          -- case erased => {
+          --   apply Or.inr; exists Constant.kindU; unfold const; simp
+          --   apply ConInfer.infer _ _; exact kindu
+          --   apply Infer.ax
+          --   apply cinfer_implies_wf j1
+          --   apply RedStar.refl
+          -- }
+        }
+        case inter => {
+          cases j; case _ A' j step =>
+          cases j; case _ S j1 j2 =>
+          -- easy
+          sorry
+        }
+      }
+      case ctor c u1 u2 u3 => {
+        simp at *
+        have s1 : size u1 ≤ s := by linarith
+        have s2 : size u2 ≤ s := by linarith
+        have s3 : size u3 ≤ s := by linarith
+        cases c <;> simp at *
+        case app m => {
+          sorry
+        }
+        case pair => sorry
+        case fst => sorry
+        case snd => sorry
+        case eq => {
+          cases j; case _ T j step =>
+          cases j; case _ j1 j2 j3 =>
+          -- easy
+          sorry
+        }
+        case refl => {
+          sorry
+        }
+        case eqind => {
+          cases j; case _ A' j step =>
+          cases j
+        }
+        case promote => sorry
+        case delta => sorry
+        case phi => sorry
+      }
+    })
+    (size t)
+    Γ
+    t
+    A
+    (by simp)
+    (ConInfer.infer j RedStar.refl)
+
+end Cedille
