Cedille/Lemma/Erasure.lean
@@ -3,114 +3,114 @@ import Common
 import Cedille.Def
 import Cedille.Lemma.Refold
 import Cedille.Lemma.Inversion
+import Cedille.Lemma.Syntax
 
 namespace Cedille
 
-  @[simp] lemma erase_bound : erase (bound i) = bound i := by congr
-  @[simp] lemma erase_free {n} : erase (@free n x) = free x := by congr
-  @[simp] lemma erase_const {n} : erase (@const n c) = const c := by congr
-  @[simp] lemma erase_typeu {n} : erase (@typeu n) = typeu := by congr
-  @[simp] lemma erase_kindu {n} : erase (@kindu n) = kindu := by congr
+  @[simp] lemma erase_bound : erase x (bound i) = bound i := by congr
+  @[simp] lemma erase_free {n} : erase z (@free n x) = free x := by congr
+  @[simp] lemma erase_const {n} : erase x (@const n c) = const c := by congr
+  @[simp] lemma erase_typeu {n} : erase x (@typeu n) = typeu := by congr
+  @[simp] lemma erase_kindu {n} : erase x (@kindu n) = kindu := by congr
   
-  @[simp] lemma erase_lam_mf : erase (lam mf a b) = lam mf kindu (erase b) := by congr
+  @[simp] lemma erase_lam_mf : erase x (lam mf a b) = lam mf kindu (erase x b) := by congr
   @[simp] lemma erase_lam_mf_unfolded
-    : erase (Syntax.bind (Binder.lam mf) a b) = lam mf kindu (erase b)
+    : erase x (Syntax.bind (Binder.lam mf) a b) = lam mf kindu (erase x b)
   := by congr
 
-  @[simp] lemma erase_lam_mt : erase (lam mt a b) = lam mt (erase a) (erase b) := by congr
+  @[simp] lemma erase_lam_mt : erase x (lam mt a b) = lam mt (erase x a) (erase x b) := by congr
   @[simp] lemma erase_lam_mt_unfolded
-    : erase (Syntax.bind (Binder.lam mt) a b) = lam mt (erase a) (erase b)
+    : erase x (Syntax.bind (Binder.lam mt) a b) = lam mt (erase x a) (erase x b)
   := by congr
 
-  @[simp] lemma erase_pi : erase (pi m a b) = pi m (erase a) (erase b) := by congr
+  @[simp] lemma erase_pi : erase x (pi m a b) = pi m (erase x a) (erase x b) := by congr
   @[simp] lemma erase_pi_unfolded
-    : erase (Syntax.bind (Binder.pi m) a b) = pi m (erase a) (erase b)
+    : erase x (Syntax.bind (Binder.pi m) a b) = pi m (erase x a) (erase x b)
   := by congr
 
-  @[simp] lemma erase_inter : erase (inter a b) = inter (erase a) (erase b) := by congr
+  @[simp] lemma erase_inter : erase x (inter a b) = inter (erase x a) (erase x b) := by congr
   @[simp] lemma erase_inter_unfolded
-    : erase (Syntax.bind Binder.inter a b) = inter (erase a) (erase b)
+    : erase x (Syntax.bind Binder.inter a b) = inter (erase x a) (erase x b)
   := by congr
 
   @[simp] lemma erase_lam_m0 {n} {a : Term n} {b : Term (n + 1)}
-    : erase (lam m0 a b) = let x := Name.fresh (fv b); erase ({_|-> x}b)
+    : erase x (lam m0 a b) = erase x ({_|-> x}b)
   := by {
     unfold lam; simp only
-    generalize erase ({_|-> Name.fresh (fv b)}b) = t
     rfl
   }
 
-  @[simp] lemma erase_app_m0 : erase (t1 @0 t2) = erase t1
+  @[simp] lemma erase_app_m0 : erase x (t1 @0 t2) = erase x t1
     := by rfl
   @[simp] lemma erase_app_m0_unfolded
-    : erase (Syntax.ctor (Constructor.app m0) t1 t2 t3) = erase t1
+    : erase x (Syntax.ctor (Constructor.app m0) t1 t2 t3) = erase x t1
   := by rfl
 
-  @[simp] lemma erase_app_mf : erase (t1 @ω t2) = (erase t1) @ω (erase t2) := by congr
+  @[simp] lemma erase_app_mf : erase x (t1 @ω t2) = (erase x t1) @ω (erase x t2) := by congr
   @[simp] lemma erase_app_mf_unfolded
-    : erase (Syntax.ctor (Constructor.app mf) t1 t2 t3) = app mf (erase t1) (erase t2)
+    : erase x (Syntax.ctor (Constructor.app mf) t1 t2 t3) = app mf (erase x t1) (erase x t2)
   := by {
-    generalize h : (erase t1) @ω (erase t2) = t
+    generalize h : (erase x t1) @ω (erase x t2) = t
     unfold erase; simp only; subst h; rfl
   }
 
-  @[simp] lemma erase_app_mt : erase (t1 @τ t2) = (erase t1) @τ (erase t2) := by congr
+  @[simp] lemma erase_app_mt : erase x (t1 @τ t2) = (erase x t1) @τ (erase x t2) := by congr
   @[simp] lemma erase_app_mt_unfolded
-    : erase (Syntax.ctor (Constructor.app mt) t1 t2 t3) = app mt (erase t1) (erase t2)
+    : erase x (Syntax.ctor (Constructor.app mt) t1 t2 t3) = app mt (erase x t1) (erase x t2)
   := by {
-    generalize h : (erase t1) @τ (erase t2) = t
+    generalize h : (erase x t1) @τ (erase x t2) = t
     unfold erase; simp only; subst h; rfl
   }
 
-  @[simp] lemma erase_pair : erase (pair t1 t2 t3) = erase t1
+  @[simp] lemma erase_pair : erase x (pair t1 t2 t3) = erase x t1
     := rfl
   @[simp] lemma erase_pair_unfolded
-    : erase (Syntax.ctor Constructor.pair t1 t2 t3) =erase t1
+    : erase x (Syntax.ctor Constructor.pair t1 t2 t3) =erase x t1
   := rfl
 
-  @[simp] lemma erase_fst : erase (fst t) = erase t := by generalize t = s; rfl
+  @[simp] lemma erase_fst : erase x (fst t) = erase x t := by generalize t = s; rfl
   @[simp] lemma erase_fst_unfolded
-    : erase (Syntax.ctor Constructor.fst t1 t2 t3) =erase t1
+    : erase x (Syntax.ctor Constructor.fst t1 t2 t3) =erase x t1
   := rfl
 
-  @[simp] lemma erase_snd : erase (snd t) = erase t := by generalize t = s; rfl
+  @[simp] lemma erase_snd : erase x (snd t) = erase x t := by generalize t = s; rfl
   @[simp] lemma erase_snd_unfolded
-    : erase (Syntax.ctor Constructor.snd t1 t2 t3) =erase t1
+    : erase x (Syntax.ctor Constructor.snd t1 t2 t3) =erase x t1
   := rfl
 
-  @[simp] lemma erase_eq : erase (eq t1 t2 t3) = eq (erase t1) (erase t2) (erase t3)
+  @[simp] lemma erase_eq : erase x (eq t1 t2 t3) = eq (erase x t1) (erase x t2) (erase x t3)
     := by congr
   @[simp] lemma erase_eq_unfolded
-    : erase (Syntax.ctor Constructor.eq t1 t2 t3) = eq (erase t1) (erase t2) (erase t3)
+    : erase x (Syntax.ctor Constructor.eq t1 t2 t3) = eq (erase x t1) (erase x t2) (erase x t3)
   := by {
-    generalize h : eq (erase t1) (erase t2) (erase t3) = t
+    generalize h : eq (erase x t1) (erase x t2) (erase x t3) = t
     unfold erase; subst h; rfl
   }
 
-  @[simp] lemma erase_refl : erase (refl t) = lam mf kindu (bound 0) := by congr
+  @[simp] lemma erase_refl : erase x (refl t) = lam mf kindu (bound 0) := by congr
   @[simp] lemma erase_refl_unfolded
-    : erase (Syntax.ctor Constructor.refl t1 t2 t3) = lam mf kindu (bound 0)
+    : erase x (Syntax.ctor Constructor.refl t1 t2 t3) = lam mf kindu (bound 0)
   := by congr
 
-  @[simp] lemma erase_eqind {n} : erase (@J n) = lam mf kindu (bound 0) := by congr
+  @[simp] lemma erase_eqind {n} : erase x (@J n) = lam mf kindu (bound 0) := by congr
   @[simp] lemma erase_eqind_unfolded
-    : erase (Syntax.ctor Constructor.eqind t1 t2 t3) = lam mf kindu (bound 0)
+    : erase x (Syntax.ctor Constructor.eqind t1 t2 t3) = lam mf kindu (bound 0)
   := by congr
 
-  @[simp] lemma erase_promote : erase (promote t) = erase t := by rfl
+  @[simp] lemma erase_promote : erase x (promote t) = erase x t := by rfl
   @[simp] lemma erase_promote_unfolded
-    : erase (Syntax.ctor Constructor.promote t1 t2 t3) = erase t1
+    : erase x (Syntax.ctor Constructor.promote t1 t2 t3) = erase x t1
   := rfl
 
-  @[simp] lemma erase_delta : erase (delta t) = erase t := by rfl
+  @[simp] lemma erase_delta : erase x (delta t) = erase x t := by rfl
   @[simp] lemma erase_delta_unfolded
-    : erase (Syntax.ctor Constructor.delta t1 t2 t3) = erase t1
+    : erase x (Syntax.ctor Constructor.delta t1 t2 t3) = erase x t1
   := by rfl
 
-  @[simp] lemma erase_phi : erase (phi t1 t2 t3) = erase t1 := by rfl
+  @[simp] lemma erase_phi : erase x (phi t1 t2 t3) = erase x t1 := by rfl
 
-  @[simp] lemma erase_idem {m} {t : Term m} : erase (erase t) = erase t := @Nat.rec
-    (λ n => {m : Nat} -> (t : Term m) -> size t ≤ n -> erase (erase t) = erase t)
+  @[simp] lemma erase_idem {m} {t : Term m} : erase y (erase x t) = erase x t := @Nat.rec
+    (λ n => {m : Nat} -> (t : Term m) -> size t ≤ n -> erase y (erase x t) = erase x t)
     (by {
       intro m t h
       cases t <;> simp <;> simp at h
@@ -119,22 +119,16 @@ namespace Cedille
       intros n ih m t h
       cases t <;> simp <;> simp at h
       case bind k t1 t2 => {
-        have h := Nat.le_of_succ_le_succ h
-        have h := nat_add_le h
-        casesm* _ ∧ _
-        case _ h1 h2 =>
+        have h1 : size t1 ≤ n := by linarith
+        have h2 : size t2 ≤ n := by linarith
         cases k <;> simp [*]
         case lam k =>
         cases k <;> simp [*]
       }
       case ctor k t1 t2 t3 => {
-        have h := Nat.le_of_succ_le_succ h
-        have h := nat_add_le h
-        casesm* _ ∧ _
-        case _ h1 _ =>
-        have h := nat_add_le h1
-        casesm* _ ∧ _
-        case _ h1 h2 =>
+        have h1 : size t1 ≤ n := by linarith
+        have h2 : size t2 ≤ n := by linarith
+        have h3 : size t3 ≤ n := by linarith
         cases k <;> simp [*]
         case app m =>
         cases m <;> simp [*]
@@ -145,40 +139,184 @@ namespace Cedille
     t
     (by simp)
 
-  lemma erase_rename : erase t1 = erase t2 -> erase ({_|-> x}{_<-| y}t1) = erase ({_|-> x}{_<-| y}t2)
-  := by sorry
+  lemma erase_rename_commute (x y z) {n} {t : Term n} (h : x ≠ z)
+    : {_|-> y}{_<-| x}(erase z t) = erase z ({_|-> y}{_<-| x}t)
+  := @Nat.rec
+    (λ s => ∀ n (t : Term n),
+      size t ≤ s ->
+      {_|-> y}{_<-| x}(erase z t) = erase z ({_|-> y}{_<-| x}t))
+    (by {
+      intro n t sh
+      cases t <;> simp at *
+      case bound i => {
+        unfold HasHOpen.hopn; unfold Syntax.instHasHOpenSyntax; simp
+        unfold Syntax.opn_head; unfold bound; simp
+        intro h
+        cases i; case _ iv il =>
+        simp at h
+        linarith
+      }
+      case free w => split <;> simp
+    })
+    (by {
+      intro s ih n t sh
+      cases t
+      case bound => apply ih _ (bound _) (by simp)
+      case free => apply ih _ (free _) (by simp)
+      case const => apply ih _ (const _) (by simp)
+      case bind k u1 u2 => {
+        simp at *
+        have s1 : size u1 ≤ s := by linarith
+        have s2 : size u2 ≤ s := by linarith
+        cases k <;> simp at *
+        case lam m => {
+          cases m <;> simp at *
+          case free => rw [ih _ u2 s2]
+          case erased => {
+            have sh : size ({_|-> z}u2) ≤ s := by simp; linarith
+            have lem := ih _ ({_|-> z}u2) sh
+            rw [lem, @rename_open_commute _ z x y u2 (ne_sym h)]
+          }
+          case type => rw [ih _ u1 s1, ih _ u2 s2]
+        }
+        case pi m => rw [ih _ u1 s1, ih _ u2 s2]
+        case inter => rw [ih _ u1 s1, ih _ u2 s2]
+      }
+      case ctor k u1 u2 u3 => {
+        simp at *
+        have s1 : size u1 ≤ s := by linarith
+        have s2 : size u2 ≤ s := by linarith
+        have s3 : size u3 ≤ s := by linarith
+        cases k <;> simp at * <;> try rw [ih _ u1 s1]
+        case app m => {
+          cases m <;> simp at *
+          case free => rw [ih _ u1 s1, ih _ u2 s2]
+          case erased => rw [ih _ u1 s1]
+          case type => rw [ih _ u1 s1, ih _ u2 s2]
+        }
+        case eq => rw [ih _ u2 s2, ih _ u3 s3]
+        case refl => {
+          unfold HasHOpen.hopn; unfold Syntax.instHasHOpenSyntax; simp
+          unfold Syntax.opn_head; unfold bound; simp
+          split <;> simp
+          exfalso; linarith
+        }
+        case eqind => {
+          unfold HasHOpen.hopn; unfold Syntax.instHasHOpenSyntax; simp
+          unfold Syntax.opn_head; unfold bound; simp
+          split <;> simp
+          exfalso; linarith
+        }
+      }
+    })
+    (size t)
+    n
+    t
+    (by simp)
 
-  lemma erase_free_rename :
-    ((x : Name) -> x ∉ fv t -> x ∉ (fv ∘ erase) ({_|-> x}t)) ->
-    (x y : Name) -> x ∉ fv t -> y ∉ fv t -> erase ({_|-> x}t) = erase ({_|-> y}t)
-  := by {
-    intro h x y xnin ynin
-    have hx := h x xnin
-    have hy := h y ynin
-    sorry
-  }
+  -- lemma erase_rename {n} {t1 t2 : Term n} : erase z t1 = erase z t2 ->
+  --   erase z ({_|-> y}{_<-| x}t1) = erase z ({_|-> y}{_<-| x}t2)
+  -- := λ h => @Nat.rec
+  --   (λ s => ∀ n (t1 t2 : Term n),
+  --     size t1 + size t2 ≤ s ->
+  --     erase x t1 = erase x t2 ->
+  --     erase x ({_|-> y}{_<-| x}t1) = erase x ({_|-> y}{_<-| x}t2))
+  --   (by {
+  --     intro n t1 t2 sh h
+  --     cases t1 <;> simp at *
+  --     case bound i => {
+  --       cases t2 <;> simp at *
+  --       case bound i' => injection h; simp [*]
+  --     }
+  --     case free z => {
+  --       cases t2 <;> simp at *
+  --       case free z' => {
+  --         injection h with _ e; subst e
+  --         split <;> simp at *
+  --       }
+  --     }
+  --     case const c => {
+  --       cases t2 <;> simp at *
+  --       case const k' => injection h; simp [*]
+  --     }
+  --   })
+  --   (by {
+  --     intro s ih n t1 t2 sh h
+  --     cases t1
+  --     case bound => sorry
+  --     case free => sorry
+  --     case const => sorry
+  --     case bind k1 u1 u2 => {
+  --       cases k1 <;> simp at *
+  --       case lam m => {
+  --         cases m <;> simp at *
+  --         case free => sorry
+  --         case erased => {
+  --           generalize zdef : Name.fresh (fv u2) = z at *
+  --           have sh : size ({_|-> z}u2) + size t2 ≤ s := by simp; linarith
+  --           have lem := ih _ ({_|-> z}u2) t2 sh h
+  --           rw [<-lem]
+  --         }
+  --         case type => sorry
+  --       }
+  --       case pi m => {
+  --         cases t2 <;> simp at *
+  --         case bind k2 v1 v2 => sorry
+  --         case ctor k2 v1 v2 v3 => {
+  --           cases k2 <;> simp at *
+  --           case app m => {
+  --             cases m <;> simp at *
+  --             case erased => {
+  --               have sh : size u1 + size u2 + 1 + size v1 ≤ s := by linarith
+  --               have lem := ih _ (pi m u1 u2) v1 sh h
+  --               rw [<-lem]; simp
+  --             }
+  --           }
+  --           repeat sorry
+  --         }
+  --       }
+  --       case inter => sorry
+  --     }
+  --     case ctor => sorry
+  --   })
+  --   (size t1 + size t2)
+  --   n
+  --   t1
+  --   t2
+  --   (by simp)
+  --   h
 
-  -- @[simp] lemma erase_subst : erase ([_:= a]f) = [_:= erase a](erase f) := sorry
+  -- lemma erase_free_rename :
+  --   ((x : Name) -> x ∉ fv t -> x ∉ (fv ∘ erase) ({_|-> x}t)) ->
+  --   (x y : Name) -> x ∉ fv t -> y ∉ fv t -> erase x ({_|-> x}t) = erase x ({_|-> y}t)
+  -- := by {
+  --   intro h x y xnin ynin
+  --   have hx := h x xnin
+  --   have hy := h y ynin
+  --   sorry
+  -- }
 
-  -- lemma erase_close_open : erase t = {_|-> x}s -> erase ({_<-| x}t) = s := sorry
+  -- @[simp] lemma erase_subst : erase x ([_:= a]f) = [_:= erase x a](erase x f) := sorry
 
-  -- lemma erase_forces_lam_mt : erase f = lam mt t1 t2 ->
-  --   ∃ t1' t2', erase t1' = t1 ∧ erase t2' = t2 ∧ f = lam mt t1' t2'
+  -- lemma erase_close_open : erase x t = {_|-> x}s -> erase x ({_<-| x}t) = s := sorry
+
+  -- lemma erase_forces_lam_mt : erase x f = lam mt t1 t2 ->
+  --   ∃ t1' t2', erase x t1' = t1 ∧ erase x t2' = t2 ∧ f = lam mt t1' t2'
   -- := sorry
 
-  -- lemma erase_forces_lam_mf : erase f = lam mf t1 t2 ->
-  --   ∃ t1' t2', erase t1' = t1 ∧ erase t2' = t2 ∧ f = lam mf t1' t2'
+  -- lemma erase_forces_lam_mf : erase x f = lam mf t1 t2 ->
+  --   ∃ t1' t2', erase x t1' = t1 ∧ erase x t2' = t2 ∧ f = lam mf t1' t2'
   -- := sorry
 
-  -- lemma erase_no_eqind : erase f ≠ J @τ t1 @τ t2 @0 t3 @0 t4 @ω t5 := sorry
+  -- lemma erase_no_eqind : erase x f ≠ J @τ t1 @τ t2 @0 t3 @0 t4 @ω t5 := sorry
 
   -- lemma erase_free_invariant :
   --   x ∉ (fv ∘ erase) ({_|-> x}t) ->
   --   (y : Name) -> y ∉ fv t ->
-  --   erase ({_|-> x}t) = erase ({_|-> y}t)
+  --   erase x ({_|-> x}t) = erase x ({_|-> y}t)
   -- := sorry
 
-  -- lemma erase_ctt_eq : erase t = erase ctt -> t = lam mf kindu (lam mf kindu (bound 0)) := sorry
-  -- lemma erase_cff_eq : erase t = erase cff -> t = lam mf kindu (lam mf kindu (bound 1)) := sorry
+  -- lemma erase_ctt_eq : erase x t = erase x ctt -> t = lam mf kindu (lam mf kindu (bound 0)) := sorry
+  -- lemma erase_cff_eq : erase x t = erase x cff -> t = lam mf kindu (lam mf kindu (bound 1)) := sorry
 
 end Cedille
