Cedille/Lemma/Preservation.lean
@@ -1,0 +1,472 @@
+
+import Common
+import Cedille.Def
+import Cedille.Lemma.Basic
+import Cedille.Lemma.Refold
+import Cedille.Lemma.Erasure
+import Cedille.Lemma.Inversion
+import Cedille.Lemma.Red
+
+namespace Cedille
+
+  lemma preservation_of_infer_step_subst :
+    Γ ⊢ lam m u1 u2 >: pi m A B ->
+    Γ ⊢ u3 =: A ->
+    ∃ B, Γ ⊢ [_:= u3]u2 : B
+  := by sorry
+
+  lemma preservation_step_of_infer_ctx (S : FvSet!) :
+    ((x : Name) -> x ∉ S → (Γ ++ [x:A]) ⊢ {_|-> x}t : {_|-> x}B) ->
+    A -β> A' ->
+    ∃ B, ((x : Name) -> x ∉ S → (Γ ++ [x:A']) ⊢ {_|-> x}t : {_|-> x}B)
+  := by sorry
+
+  lemma preservation_step_of_cinfer_ctx (S : FvSet!) :
+    ((x : Name) -> x ∉ S → (Γ ++ [x:A]) ⊢ {_|-> x}t >: {_|-> x}B) ->
+    A -β> A' ->
+    ((x : Name) -> x ∉ S → (Γ ++ [x:A']) ⊢ {_|-> x}t >: {_|-> x}B)
+  := by sorry
+
+  lemma preservation_step_of_cinfer_ctx_const (S : FvSet!) :
+    ((x : Name) -> x ∉ S → (Γ ++ [x:A]) ⊢ {_|-> x}t >: const K) ->
+    A -β> A' ->
+    ((x : Name) -> x ∉ S → (Γ ++ [x:A']) ⊢ {_|-> x}t >: const K)
+  := by sorry
+
+  lemma rule_cinfer_red : Γ ⊢ t >: A -> A -β>* B -> Γ ⊢ t >: B := by {
+    intro j step
+    cases j; case _ D j step2 =>
+    replace step := RedStar.trans step2 step
+    apply ConInfer.infer j step
+  }
+
+  lemma rule_inv_inter1_kind : ¬ (Γ ⊢ t >: inter (const K) B) := λ j => @Nat.rec
+    (λ s => ∀ Γ t K B,
+      size t ≤ s ->
+      ¬ Γ ⊢ t >: inter (const K) B)
+    sorry
+    (by {
+      intro s ih Γ t K B sh j
+      cases t <;> simp at *
+      case bound => apply ih _ (bound _) _ _ (by simp) j
+      case free => apply ih _ (free _) _ _ (by simp) j
+      case const => apply ih _ (const _) _ _ (by simp) j
+      case bind b u1 u2 => {
+        cases b <;> simp at *
+        case lam m => {
+          sorry
+        }
+        case pi m => sorry
+        case inter => sorry
+      }
+      case ctor => sorry
+    })
+    (size t)
+    Γ
+    t
+    K
+    B
+    (by simp)
+    j
+
+  lemma preservation_step_of_cinfer_const :
+    Γ ⊢ t >: const K ->
+    t -β> s ->
+    Γ ⊢ s >: const K
+  := λ j step => @ConInfer.rec
+    (λ Γ t A j => ∀ s K, A -β>* const K -> t -β> s -> Γ ⊢ s : A)
+    (λ Γ t A j => ∀ s K, A = const K -> t -β> s -> Γ ⊢ s >: A)
+    (λ Γ t A j => ∀ s K, A = const K -> t -β> s -> Γ ⊢ s =: A)
+    (λ Γ wf => True)
+    (by {
+      intro Γ wf _ s K e step
+      cases step
+    })
+    (by {
+      intro Γ x A wf xn _ s K e step
+      cases step
+    })
+    (by {
+      intro Γ A m K B S j1 j2 ih1 ih2 s K' e step; simp at *
+      cases step <;> simp at *
+      case bind1 A' step => {
+        cases m <;> simp at *
+        case free => {
+          have lem1 := ih1 A' Constant.typeU rfl step
+          have lem2 := preservation_step_of_cinfer_ctx_const S j2 step
+          apply @Infer.pi _ _ mf Constant.typeU _ _ lem1 lem2
+        }
+        case erased => {
+          have lem1 := ih1 A' K rfl step
+          have lem2 := preservation_step_of_cinfer_ctx_const S j2 step
+          apply @Infer.pi _ _ m0 K _ _ lem1 lem2
+        }
+        case type => {
+          have lem1 := ih1 A' K rfl step
+          have lem2 := preservation_step_of_cinfer_ctx_const S j2 step
+          apply @Infer.pi _ _ mt K _ _ lem1 lem2
+        }
+      }
+      case bind2 B' S' step => {
+        cases m <;> simp at *
+        case free => {
+          have lem2 : ∀ x, x ∉ (S ++ S') -> (Γ ++ [x:A]) ⊢ {_|-> x}B' >: typeu := by {
+            intro x xn; simp at xn
+            replace xn := demorgan xn
+            cases xn; case _ xn1 xn2 =>
+            apply ih2 x xn1 ({_|-> x}B') Constant.typeU rfl _
+            apply step x xn2
+          }
+          apply @Infer.pi _ _ mf Constant.typeU _ (S ++ S') j1 lem2
+        }
+        case erased => {
+          have lem2 : ∀ x, x ∉ (S ++ S') -> (Γ ++ [x:A]) ⊢ {_|-> x}B' >: typeu := by {
+            intro x xn; simp at xn
+            replace xn := demorgan xn
+            cases xn; case _ xn1 xn2 =>
+            apply ih2 x xn1 ({_|-> x}B') Constant.typeU rfl _
+            apply step x xn2
+          }
+          apply @Infer.pi _ _ m0 K _ (S ++ S') j1 lem2
+        }
+        case type => {
+          have lem2 : ∀ x, x ∉ (S ++ S') -> (Γ ++ [x:A]) ⊢ {_|-> x}B' >: kindu := by {
+            intro x xn; simp at xn
+            replace xn := demorgan xn
+            cases xn; case _ xn1 xn2 =>
+            apply ih2 x xn1 ({_|-> x}B') Constant.kindU rfl _
+            apply step x xn2
+          }
+          apply @Infer.pi _ _ mt K _ (S ++ S') j1 lem2
+        }
+      }
+    })
+    sorry
+    sorry
+    sorry
+    (sorry)
+    (by {
+      intro Γ t A B j ih s K e step
+      sorry
+    })
+    sorry
+    (by {
+      intro Γ A a b j1 j2 j3 ih1 ih2 ih3 s K e step
+      cases step <;> simp at *
+      case ctor1 => sorry
+      case ctor2 a' step => {
+        sorry
+      }
+      case ctor3 => sorry
+    })
+    sorry
+    sorry
+    sorry
+    sorry
+    sorry
+    (by {
+      intro Γ t A B j step ih s K e step'
+      subst e
+      have lem := ih s K step step'
+      apply ConInfer.infer lem step
+    })
+    (by {
+      intro Γ t A B K' j1 j2 conv ih1 ih2 s K e step
+      subst e;
+      cases conv; case _ A' K' S s1 er s2 =>
+      cases s2
+      case refl => {
+        clear ih2
+        sorry
+      }
+      case step _ step _ => cases step
+    })
+    (by simp)
+    (by simp)
+    Γ
+    t
+    (const K)
+    j
+    s
+    K
+    rfl
+    step
+
+
+  lemma preservation_step_of_cinfer_pi_domain :
+    Γ ⊢ t >: Mode.pi_domain m K ->
+    t -β> s ->
+    Γ ⊢ s >: Mode.pi_domain m K
+  := λ j step => @Nat.rec
+    (λ si => ∀ Γ t m K s,
+      size t ≤ si ->
+      Γ ⊢ t >: Mode.pi_domain m K ->
+      t -β> s ->
+      Γ ⊢ s >: Mode.pi_domain m K)
+    sorry
+    (by {
+      intro si ih Γ t m K s sh j step
+      cases t <;> simp at *
+      case bound => cases step
+      case free => cases step
+      case const => cases step
+      case bind b u1 u2 => {
+        have s1 : size u1 ≤ si := by linarith 
+        have s2 : size u2 ≤ si := by linarith
+        cases b <;> simp at *
+        case lam m' => {
+          cases j; case _ D j step2 =>
+          cases j; case _ K2 B2 S2 j1 j2 j3 =>
+          exfalso; apply red_inv_pi_not_pi_domain step2
+        }
+        case pi m' => {
+          cases j; case _ D j step2 =>
+          cases j; case _ K2 S2 j1 j2 =>
+          have e := red_force_mode_pi_codomain step2; rw [e]
+          cases step <;> simp
+          case bind1 u1' step => {
+            cases m' <;> simp at *
+            case free => {
+              have lem := @ih Γ u1 mf Constant.typeU u1' s1 j1 step; simp at lem
+              apply ConInfer.infer _ _; exact typeu
+              apply @Infer.pi _ _ mf Constant.typeU _ S2 lem
+              simp; apply preservation_step_of_cinfer_ctx_const S2 j2 step
+              apply RedStar.refl
+            }
+            case erased => sorry
+            case type => sorry
+          }
+          case bind2 => sorry
+        }
+        case inter => {
+          cases j; case _ D j step2 =>
+          cases j; case _ S2 j1 j2 =>
+          have e := red_force_typeu step2; rw [e]
+          cases step <;> simp
+          case bind1 u1' step => {
+            have lem := @ih Γ u1 mf K u1' s1 j1 step; simp at lem
+            sorry
+          }
+          case bind2 => sorry
+        }
+      }
+      case ctor c u1 u2 u3 => {
+        have s1 : size u1 ≤ si := by linarith 
+        have s2 : size u2 ≤ si := by linarith
+        have s3 : size u3 ≤ si := by linarith
+        cases c <;> simp at *
+        case app m => sorry
+        case pair => {
+          cases j; case _ D j step2 =>
+          cases j; case _ A B j1 j2 j3 j4 =>
+          exfalso; apply red_inv_inter_not_pi_domain step2
+        }
+        case fst => {
+          cases j; case _ D j step2 =>
+          cases j; case _ B j =>
+          have step2 : inter D B -β>* inter (Mode.pi_domain m K) B := by {
+            apply red_inter' step2 (λ _ _ => RedStar.refl); exact []
+          }
+          replace j := rule_cinfer_red j step2
+          cases m <;> simp at *
+          case free => exfalso; apply rule_inv_inter1_kind j
+          case erased => exfalso; apply rule_inv_inter1_kind j
+          case type => exfalso; apply rule_inv_inter1_kind j
+        }
+        case snd => sorry
+        case eq => sorry
+        case refl => sorry
+        case eqind => sorry
+        case promote => sorry
+        case delta => sorry
+        case phi => sorry
+      }
+    })
+    (size t)
+    Γ
+    t
+    m
+    K
+    s
+    (by simp)
+    j
+    step
+
+
+  lemma preservation_of_infer_step4 : Γ ⊢ t : A -> t -β> s -> Γ ⊢ s : A := by {
+    intro j step
+    induction step generalizing Γ A
+    case beta m u1 u2 u3 => {
+      cases j; case _ A B S j1 j2 =>
+      sorry
+    }
+    case fst u1 u2 u3 => {
+      cases j; case _ B j =>
+      cases j; case _ T j step =>
+      sorry
+    }
+    case snd => sorry
+    case eqind => sorry
+    case promote => sorry
+    case phi => sorry
+    case bind1 => sorry
+    case bind2 => sorry
+    case ctor1 => sorry
+    case ctor2 => sorry
+    case ctor3 => sorry
+  }
+
+  lemma preservation_of_infer_step : Γ ⊢ t : A -> t -β> s -> ∃ B, Γ ⊢ s : B := by {
+    intro tproof step
+    induction step generalizing Γ A
+    case beta m u1 u2 u3 => {
+      cases tproof; case _ A B S j1 j2 =>
+      apply preservation_of_infer_step_subst j1 j2
+    }
+    case fst u1 u2 u3 => {
+      cases tproof; case _ B j =>
+      cases j; case _ P j step =>
+      cases j; case _ A2 B2 j1 j2 j3 j4 =>
+      cases j1; case _ A3 j5 j6 =>
+      sorry
+    }
+    case snd u1 u2 u3 => {
+      cases tproof; case _ A1 B1 j =>
+      cases j; case _ P j1 s1 =>
+      cases j1; case _ A2 B2 j1 j2 j3 j4 =>
+      cases j3; case _ A3 j5 c1 =>
+      sorry
+    }
+    case eqind u1 u2 u3 u4 u5 u6 => {
+      cases tproof
+      case app A1 B1 S1 j1 j2 => {
+        cases j1; case _ D1 j1 s1 =>
+        cases j1; case _ A2 B2 S2 j4 j5 =>
+        cases j4; case _ D2 j4 s2 =>
+        cases j4; case _ A3 B3 S3 j6 j7 =>
+        cases j6; case _ D3 j6 s3 =>
+        cases j6; case _ A4 B4 S4 j8 j9 =>
+        cases j8; case _ D4 j8 s4 =>
+        cases j8; case _ A5 B5 S5 j8 j11 =>
+        cases j8; case _ D5 j8 s5 =>
+        cases j8; case _ A6 B6 S6 j8 j13 =>
+        cases j8; case _ D6 j8 s6 => 
+        cases j8
+      }
+      case eqind j1 j2 j3 j4 j5 j6 => {
+        cases j5; case _ D j5 c1 =>
+        cases j5; case _ A j =>
+        sorry
+      }
+    }
+    case promote u => {
+      cases tproof; case _ T a b A B j1 j2 =>
+      cases j2; case _ A2 j2 s1 =>
+      cases j2; case _ A3 j2 =>
+      cases j2; case _ B2 j2 =>
+      cases j2; case _ T j s2 =>
+      exists eq T u u
+      apply Infer.refl; simp [*]
+    }
+    case phi u1 u2 u3 S er => {
+      cases tproof; case _ A B S j1 j2 f1 f2 j3 =>
+      cases j2; case _ T j2 s1 =>
+      exists T
+    }
+    case bind1 u1 u2 k u3 s1 ih => {
+      cases k <;> simp at *
+      case lam m => {
+        cases tproof; case _ K B S j1 j2 j3 =>
+        cases j1; case _ T j1 step2 =>
+        have lem := ih j1
+        cases lem; case _ D jlem =>
+        have cj1 : Γ ⊢ u1 >: Mode.pi_domain m K := ConInfer.infer j1 step2
+        have lem1 := preservation_step_of_cinfer_pi_domain cj1 s1
+        have lem2 := @preservation_step_of_infer_ctx Γ u1 u3 B u2 S j3 s1
+        cases lem2; case _ B' lem2 =>
+        exists (pi m u2 B')
+        apply Infer.lam lem1 lem2 j2
+      }
+      case pi m => sorry
+      case inter => sorry
+    }
+    case bind2 u1 u2 k u3 S1 s1 ih => {
+      cases k <;> simp at *
+      case lam m => {
+        cases tproof; case _ K B S2 j1 j2 j3 =>
+        have xfresh := @Name.fresh_is_fresh (S1 ++ S2)
+        generalize xdef : Name.fresh (S1 ++ S2) = x at *
+        simp at *
+        replace xfresh := demorgan xfresh
+        cases xfresh; case _ xn1 xn2 =>
+        have lem1 := ih x xn1 (j3 x xn2)
+        cases lem1; case _ D lem1 =>
+        have lem2 := to_open D x
+        cases lem2; case _ D' lem2 =>
+        subst lem2
+        exists pi m u3 D'
+        apply Infer.lam j1 _ _
+        exact S2; intro y yn
+        sorry
+
+
+        sorry
+      }
+      case pi m => sorry
+      case inter => sorry
+    }
+    case ctor1 => sorry
+    case ctor2 => sorry
+    case ctor3 => sorry
+  }
+
+  lemma preservation_of_infer_step3 : Γ ⊢ t : A -> t -β> s -> ∃ B, Γ ⊢ s : B
+    := λ j step => @Infer.rec
+      (λ Γ t A j' => ∀ s, t -β> s -> ∃ B, Γ ⊢ s : B)
+      (λ Γ t A j' => ∀ s, t -β> s -> ∃ B, Γ ⊢ s >: B)
+      (λ Γ t A j' => ∀ s, t -β> s -> ∃ B, Γ ⊢ s =: B)
+      (λ Γ wf => True)
+    sorry
+    sorry
+    sorry
+    (by {
+      intro Γ A m K t B S j1 j2 j3 ih1 ih2 s step; simp at *
+      cases step <;> simp
+      case bind1 A' step => {
+        sorry
+      }
+      case bind2 => sorry
+    })
+    sorry
+    sorry
+    sorry
+    sorry
+    sorry
+    sorry
+    sorry
+    sorry
+    sorry
+    sorry
+    sorry
+    (by {
+      intro Γ t A B j step ih s step2
+      have lem := ih s step2
+      cases lem; case _ D j2 =>
+      sorry
+    })
+    (by {
+      intro Γ t A B j c ih s step
+      sorry
+    })
+    sorry
+    sorry
+    Γ
+    t
+    A
+    j
+    s
+    step
+
+  theorem preservation_of_infer : Γ ⊢ t : A -> t -β>* s -> ∃ B, Γ ⊢ s : B := sorry 
+
+end Cedille
