Cedille/Lemma/Red.lean
@@ -3,6 +3,7 @@ import Cedille.Def
 import Cedille.Lemma.Basic
 import Cedille.Lemma.Refold
 import Cedille.Lemma.Erasure
+import Cedille.Lemma.Inversion
 import Cedille.Lemma.Syntax
 
 namespace Cedille
@@ -19,53 +20,8 @@ namespace Cedille
   -- }
 
 
-  lemma red_open_forced_step : {_|-> x}t1 -β> t2 -> ∃ z, t2 = {_|-> x}z ∧ x ∉ fv z := sorry
-  lemma red_open_forced : {_|-> x}t1 -β>* t2 -> ∃ z, t2 = {_|-> x}z ∧ x ∉ fv z := sorry
-
-
-  lemma red_pi : A -β>* A' -> {_|-> x}B -β>* {_|-> x}B' -> pi m A B -β>* pi m A' B' := by {
-    intro s1 s2
-    induction s1
-    case refl A => {
-      generalize Cdef1 : {_|-> x}B = C at *    
-      generalize Cdef2 : {_|-> x}B' = C' at *    
-      induction s2 generalizing x B B'
-      case refl => sorry
-      case step v1 v2 v3 vs s2 ih2 => {
-        rw [<-Cdef1] at vs
-        have e := red_open_forced_step vs
-        casesm* ∃ _, _, _ ∧ _; case _ z ze zn =>
-        have ze : {_|-> x}z = v2 := by rw [ze]
-        have lem := ih2 ze Cdef2
-        rw [<-ze] at vs
-        sorry
-      }
-    }
-    case step u1 u2 u3 us s1 ih1 => {
-      have s3 : pi m u1 B -β> pi m u2 B := by {
-        unfold pi; apply Red.bind1 us
-      }
-      apply RedStar.step s3 ih1
-    }
-  }
-
-  lemma red_lam : A -β>* A' -> {_|-> x}B -β>* {_|-> x}B' -> lam m A B -β>* lam m A' B' := sorry
-
-  lemma red_app : f -β>* f' -> a -β>* a' -> app m f a -β>* app m f' a' := sorry
-
-  lemma red_inter : A -β>* A' -> {_|-> x}B -β>* {_|-> x}B' -> inter A B -β>* inter A' B' := sorry
-
-  lemma red_pair : t -β>* t' -> s -β>* s' -> a -β>* a' -> pair t s a -β>* pair t' s' a' := sorry
-
-  lemma red_fst : t -β>* t' -> fst t -β>* fst t' := sorry
-
-  lemma red_snd : t -β>* t' -> snd t -β>* snd t' := sorry
-
-  lemma red_eq : A -β>* A' -> a -β>* a' -> b -β>* b' -> eq A a b -β>* eq A' a' b' := sorry
-
-  lemma red_promote : t -β>* t' -> promote t -β>* promote t' := sorry
-
-  lemma red_phi : a -β>* a' -> b -β>* b' -> e -β>* e' -> phi a b e -β>* phi a' b' e' := sorry
+  -- lemma red_open_forced_step : {_|-> x}t1 -β> t2 -> ∃ z, t2 = {_|-> x}z ∧ x ∉ fv z := sorry
+  -- lemma red_open_forced : {_|-> x}t1 -β>* t2 -> ∃ z, t2 = {_|-> x}z ∧ x ∉ fv z := sorry
 
   -- lemma red_open_erase : {_|-> x}(erase t) -β> s -> erase ({_|-> x}t) -β> s := sorry
 
@@ -102,25 +58,25 @@ namespace Cedille
     intros h
     induction h <;> simp [*]
     case beta t1 t2 t3 => {
-      apply And.intro _ _
-      apply subset_right; apply subset_right; simp
-      apply subset_right; apply subset_left; simp
+      apply FvSet.subset_right _
+      apply FvSet.subset_comm _
+      apply @fv_subst _ t3 t2
     }
     case snd z1 z2 z3 => {
-      apply subset_right; apply subset_left; simp
+      apply FvSet.subset_right; apply FvSet.subset_left; simp
     }
     case eqind z1 z2 z3 z4 z5 z6 => {
       apply And.intro _ _
-      apply subset_right; apply subset_right; apply subset_right;
-      apply subset_right; apply subset_right; simp
-      apply subset_right; apply subset_right; apply subset_right;
-      apply subset_right; apply subset_left; simp
+      apply FvSet.subset_right; apply FvSet.subset_right; apply FvSet.subset_right;
+      apply FvSet.subset_right; apply FvSet.subset_right; simp
+      apply FvSet.subset_right; apply FvSet.subset_right; apply FvSet.subset_right;
+      apply FvSet.subset_right; apply FvSet.subset_left; simp
     }
     case phi z1 z2 z3 => {
-      apply subset_right; apply subset_left; simp
+      apply FvSet.subset_right; apply FvSet.subset_left; simp
     }
     case bind1 z1 z2 k z3 h ih => {
-      apply subset_left; simp [*]
+      apply FvSet.subset_left; simp [*]
     }
     case bind2 z1 z2 k z3 S h ih => {
       have fresh := @Name.fresh_is_fresh (S ++ fv z2)
@@ -128,20 +84,21 @@ namespace Cedille
       have xn1 := FvSet.not_mem_left fresh
       have xn2 := FvSet.not_mem_right fresh
       have lem := ih x xn1; simp at lem
-      apply subset_right; apply subset_cons xn2 lem
+      replace lem := fv_open_shrink xn2 lem
+      apply FvSet.subset_right; exact lem
     }
     case ctor1 z1 z2 k z4 z5 h ih => {
-      apply subset_left; simp [*]
+      apply FvSet.subset_left; simp [*]
     }
     case ctor2 z1 z2 k z4 z5 h ih => {
       apply And.intro _ _
-      apply subset_right; apply subset_left; simp [*]
-      apply subset_right; apply subset_right; simp
+      apply FvSet.subset_right; apply FvSet.subset_left; simp [*]
+      apply FvSet.subset_right; apply FvSet.subset_right; simp
     }
     case ctor3 z1 z2 k z4 z5 h ih => {
       apply And.intro _ _
-      apply subset_right; apply subset_left; simp
-      apply subset_right; apply subset_right; simp [*]
+      apply FvSet.subset_right; apply FvSet.subset_left; simp
+      apply FvSet.subset_right; apply FvSet.subset_right; simp [*]
     }
   }
 
@@ -165,9 +122,14 @@ namespace Cedille
       case snd => apply Red.snd
       case eqind => apply Red.eqind
       case promote => apply Red.promote
-      case phi h => {
-        apply Red.phi
-        apply erase_rename h
+      case phi t1 t2 t3 S ih => {
+        apply Red.phi _
+        exact [x] ++ S; intro z zn; simp at *
+        replace zn := demorgan zn
+        cases zn; case _ zn1 zn2 =>
+        rw [<-erase_rename_commute x y z (ne_sym zn1)]
+        rw [<-erase_rename_commute x y z (ne_sym zn1)]
+        rw [ih z zn2]
       }
       case bind1 u1 u1' k u2 _ ih => {
         apply Red.bind1
@@ -188,81 +150,32 @@ namespace Cedille
     }
     case isTrue h => subst h; simp [*]
   }
-  --   intro yn step
-  --   cases Name.decEq x y
-  --   case isFalse h => {
-  --     induction step <;> simp
-  --     case beta m u1 u2 u3 => apply Red.beta
-  --     case fst => apply Red.fst
-  --     case snd => apply Red.snd
-  --     case eqind => apply Red.eqind
-  --     case promote => apply Red.promote
-  --     case phi h => {
-  --       apply Red.phi
-  --       apply erase_rename h
-  --     }
-  --     case bind1 u1 u1' k u2 _ ih => {
-  --       simp at yn
-  --       replace yn := demorgan yn
-  --       cases yn; case _ yn1 yn2 =>
-  --       apply Red.bind1
-  --       apply ih yn1
-  --     }
-  --     case bind2 u2 u2' k u1 S _ ih => {
-  --       simp at yn
-  --       replace yn := demorgan yn
-  --       cases yn; case _ yn1 yn2 =>
-  --       apply Red.bind2 _; exact (S ++ [x] ++ [y])
-  --       intro z zn
-  --       simp at zn
-  --       replace zn := demorgan zn
-  --       cases zn; case _ zn1 zn2 =>
-  --       replace zn2 := demorgan zn2
-  --       cases zn2; case _ zn2 zn3 =>
-  --       rw [rename_open_commute zn2, rename_open_commute zn2]
-  --       apply ih z zn1 _
-  --       simp; intro h; cases h
-  --       case _ h => subst h; apply zn3 rfl
-  --       case _ h => apply yn2 h
-  --     }
-  --     case ctor1 t1 t1' c t2 t3 _ ih => {
-  --       simp at yn
-  --       replace yn := demorgan yn; cases yn; case _ yn1 yn2 =>
-  --       replace yn2 := demorgan yn2; cases yn2; case _ yn2 yn3 =>
-  --       apply Red.ctor1; apply ih yn1
-  --     }
-  --     case ctor2 t2 t2' c t1 t3 _ ih => {
-  --       simp at yn
-  --       replace yn := demorgan yn; cases yn; case _ yn1 yn2 =>
-  --       replace yn2 := demorgan yn2; cases yn2; case _ yn2 yn3 =>
-  --       apply Red.ctor2; apply ih yn2
-  --     }
-  --     case ctor3 t3 t3' c t1 t3 _ ih => {
-  --       simp at yn
-  --       replace yn := demorgan yn; cases yn; case _ yn1 yn2 =>
-  --       replace yn2 := demorgan yn2; cases yn2; case _ yn2 yn3 =>
-  --       apply Red.ctor3; apply ih yn3
-  --     }
-  --   }
-  --   case isTrue h => subst h; simp [*]
-  -- }
 
-
-  lemma red_subst_step (x) (t : Term 0) : t1 -β> t2 -> [x := t]t1 -β> [x := t]t2 := by {
-    intro step
-    induction step
-    repeat sorry
-  }
-
-  lemma red_subst (x) (t : Term 0) : t1 -β>* t2 -> [x := t]t1 -β>* [x := t]t2 := by {
+  lemma red_rename : t1 -β>* t2 -> {_|-> y}{_<-| x}t1 -β>* {_|-> y}{_<-| x}t2 := by {
     intro step
     induction step
     case refl => apply RedStar.refl
-    case step u1 u2 u3 s1 _s2 ih => {
-      have s3  := red_subst_step x t s1
-      apply RedStar.step s3 ih
+    case step u u' v s1 _s2 ih => {
+      have lem := @red_rename_step _ _ y x s1
+      apply RedStar.step lem ih
     }
   }
+
+  -- lemma red_subst_step (x) (t : Term 0) : t1 -β> t2 -> [x := t]t1 -β> [x := t]t2 := by {
+  --   intro step
+  --   induction step
+  --   repeat sorry
+  -- }
+
+  -- lemma red_subst (x) (t : Term 0) : t1 -β>* t2 -> [x := t]t1 -β>* [x := t]t2 := by {
+  --   intro step
+  --   induction step
+  --   case refl => apply RedStar.refl
+  --   case step u1 u2 u3 s1 _s2 ih => {
+  --     have s3  := red_subst_step x t s1
+  --     apply RedStar.step s3 ih
+  --   }
+  -- }
 
   lemma red_open_generalize_step :
     x ∉ fv t1 ->
@@ -274,118 +187,18 @@ namespace Cedille
     have step2 := @red_rename_step _ _ y x step
     rw [close_open_cancel xn1, close_open_cancel xn2] at step2
     apply step2
-
-    -- intro xn1 xn2 step y yn1 yn2
-    -- generalize z1def : {_|-> x}t1 = z1 at *    
-    -- generalize z2def : {_|-> x}t2 = z2 at *
-    -- induction step generalizing t1 t2 x y
-    -- case beta => sorry
-    -- case fst u1 u2 u3 => {
-    --   cases t1 <;> unfold fst at z1def <;> simp at *
-    --   case bound => sorry
-    --   case ctor k v1 v2 v3 => {
-    --     unfold fst at z1def; injection z1def with _ e1 e2 e3 e4
-    --     have e3 : v2 = kindu := sorry
-    --     have e4 : v3 = kindu := sorry
-    --     subst e1; subst e3; subst e4; simp
-    --     cases v1 <;> simp at *
-    --     case bound => sorry
-    --     case ctor k2 w1 w2 w3 h => {
-    --       sorry
-    --       -- unfold pair at e2; injection e2 with _ e1 e2 e3 e4
-    --       -- subst e1; simp
-    --       -- rw [<-e2] at z2def
-    --       -- have e5 : t2 = w1 := sorry
-    --       -- subst e5
-    --       -- exists []; intro y yn
-    --       -- apply Red.fst
-    --     }
-    --   }
-    -- }
-    -- case snd => sorry
-    -- case eqind => sorry
-    -- case promote => sorry
-    -- case phi => sorry
-    -- case bind1 => sorry
-    -- case bind2 u1 u2 k u3 S h ih => {
-    --   cases t1 <;> simp at *
-    --   case bound => sorry
-    --   case bind b v1 v2 => {
-    --     cases t2 <;> simp at *
-    --     case bound => sorry
-    --     case bind b' w1 w2 => {
-    --       replace xn1 := demorgan xn1
-    --       replace xn2 := demorgan xn2
-    --       replace yn1 := demorgan yn1
-    --       replace yn2 := demorgan yn2
-    --       casesm* ∃ _, _, _ ∧ _; case _ e1 e2 e3 e4 e5 e6 e7 e8 e9 e10 e11 e12 e13 e14 =>
-    --       subst e1; subst e2
-    --       have e11' := open_to_close e3 e11
-    --       have e13' := open_to_close e5 e13
-    --       rw [e11', e13']
-    --       apply Red.bind2 _
-    --       exact S
-    --       intro z zn
-    --       have lem := @ih z zn z ({_|-> y}v2) ({_|-> y}w2) sorry sorry z sorry sorry
-    --       --have lem := @ih z zn z ({_|-> x}v2) ({_|-> x}w2) sorry sorry (by congr) (by congr)
-    --       --cases lem; case _ S' lem =>
-
-
-
-    --       -- casesm* ∃ _, _, _ ∧ _; case _ e1 e2 e3 e4 e5 e6 =>
-    --       -- subst e1; subst e2
-    --       -- exists S; intro y yn
-    --       -- have e1' : v2 = {_<-| x}u1 := sorry
-    --       -- have e2' : w2 = {_<-| x}u2 := sorry
-    --       -- rw [e1', e2']
-    --       -- apply Red.bind2 _
-    --       -- trivial; intro z zn
-
-
-    --     }
-    --   }
-    -- }
-    -- case ctor1 => sorry
-    -- case ctor2 => sorry
-    -- case ctor3 => sorry
   }
 
-  lemma red_open_generalize (S : FvSet!) :
+  lemma red_open_generalize :
     x ∉ fv t1 ->
     x ∉ fv t2 ->
     {_|-> x}t1 -β>* {_|-> x}t2 ->
-    ∀ y, y ∉ S -> {_|-> y}t1 -β>* {_|-> y}t2
+    ∀ y, {_|-> y}t1 -β>* {_|-> y}t2
   := by {
-    intro xn1 xn2 step
-    generalize z1def : {_|-> x}t1 = z1 at *    
-    generalize z2def : {_|-> x}t2 = z2 at *
-    induction step generalizing t1 t2 x
-    case refl t => {
-      sorry
-    }
-    case step u1 u2 u3 s1 s2 ih => {
-      rw [<-z1def] at s1
-      have s1' := red_open_forced_step s1
-      casesm* ∃ _, _, _ ∧ _; case _ z ze zn =>
-      rw [ze] at s1
-      have lem := ih zn xn2 (by rw [ze]) z2def
-      sorry
-    }
-  }
-
-  lemma red_pi2 : x ∉ fv B ++ fv B' -> {_|-> x}B -β> {_|-> x}B' -> pi m A B -β> pi m A B' := by {
-    intro xn h
-    simp at xn
-    replace xn := demorgan xn
-    cases xn; case _ xn1 xn2 =>
-    apply Red.bind2 _
-    exact (fv B ++ fv B')
-    intro y yn
-    simp at yn
-    replace yn := demorgan yn
-    cases yn; case _ yn1 yn2 =>
-    have g := red_open_generalize_step xn1 xn2 h
-    apply g y yn1 yn2
+    intro xn1 xn2 step y
+    have step2 := @red_rename _ _ y x step
+    rw [close_open_cancel xn1, close_open_cancel xn2] at step2
+    apply step2
   }
 
   namespace RedStar
@@ -399,6 +212,247 @@ namespace Cedille
       }
     }
   end RedStar
+
+  lemma red_bind1 : A -β>* A' -> Syntax.bind k A B -β>* Syntax.bind k A' B := by {
+    intro h
+    induction h
+    case refl A => apply RedStar.refl 
+    case step A A' C s1 _s2 ih => {
+      apply RedStar.step _ ih
+      apply Red.bind1 s1
+    }
+  }
+
+  lemma red_bind2 :
+    x ∉ fv B ++ fv B' ->
+    {_|-> x}B -β>* {_|-> x}B' ->
+    Syntax.bind k A B -β>* Syntax.bind k A B'
+  := by {
+    intro xn h
+    generalize C1def : {_|-> x}B = C at *
+    generalize C2def : {_|-> x}B' = C' at *
+    induction h generalizing B B'
+    case refl t => {
+      simp at xn
+      replace xn := demorgan xn
+      cases xn; case _ xn1 xn2 =>
+      replace C1def := open_to_close xn1 C1def
+      replace C2def := open_to_close xn2 C2def
+      subst C1def; subst C2def
+      apply RedStar.refl
+    }
+    case step u v u' s1 _s2 ih => {
+      simp at xn
+      replace xn := demorgan xn
+      cases xn; case _ xn1 xn2 =>
+      apply RedStar.step _ _; exact Syntax.bind k A ({_<-| x}v)
+      apply Red.bind2 _; exact []; intro y yn
+      rw [<-C1def] at s1
+      have lem := @red_rename_step _ _ y x s1
+      rw [close_open_cancel xn1] at lem
+      exact lem
+      have xn3 : x ∉ fv ({_<-| x}v) ++ fv B' := by {
+        simp; intro h
+        cases h
+        case _ h => {
+          have lem := @var_not_in_close x _ v
+          apply lem h
+        }
+        case _ h => apply xn2 h
+      }
+      apply @ih ({_<-| x}v) B' xn3 (by simp) C2def
+    }
+  }
+
+  lemma red_bind2' {S : FvSet!} :
+    ((x : Name) -> x ∉ S -> {_|-> x}B -β>* {_|-> x}B') ->
+    Syntax.bind k A B -β>* Syntax.bind k A B'
+  := by {
+    intro h
+    have fresh := @Name.fresh_is_fresh (S ++ fv B ++ fv B')
+    generalize _xdef : Name.fresh (S ++ fv B ++ fv B') = x at *
+    simp at fresh
+    replace fresh := demorgan fresh
+    cases fresh; case _ xn1 xn2' =>
+    have xn2 := demorgan xn2'
+    cases xn2; case _ xn2 xn3 =>
+    have h2 := h x xn1
+    apply red_bind2 (by simp; exact xn2') h2
+  }
+
+  lemma red_bind :
+    A -β>* A' ->
+    x ∉ fv B ++ fv B' ->
+    {_|-> x}B -β>* {_|-> x}B' ->
+    Syntax.bind k A B -β>* Syntax.bind k A' B'
+  := by {
+    intro s1 xn s2
+    apply RedStar.trans _ _; exact Syntax.bind k A' B
+    apply red_bind1 s1
+    apply red_bind2 xn s2
+  }
+
+  lemma red_bind' {S : FvSet!} :
+    A -β>* A' ->
+    ((x : Name) -> x ∉ S -> {_|-> x}B -β>* {_|-> x}B') ->
+    Syntax.bind k A B -β>* Syntax.bind k A' B'
+  := by {
+    intro s1 s2
+    apply RedStar.trans _ _; exact Syntax.bind k A' B
+    apply red_bind1 s1
+    apply red_bind2' s2
+  }
+
+  lemma red_ctor1 : A -β>* A' -> Syntax.ctor k A B C -β>* Syntax.ctor k A' B C := by {
+    intro step
+    induction step
+    case refl => apply RedStar.refl
+    case step A A' z s1 _s2 ih => {
+      apply RedStar.step _ _; exact Syntax.ctor k A' B C
+      apply Red.ctor1 s1; apply ih
+    }
+  }
+
+  lemma red_ctor2 : B -β>* B' -> Syntax.ctor k A B C -β>* Syntax.ctor k A B' C := by {
+    intro step
+    induction step
+    case refl => apply RedStar.refl
+    case step B B' z s1 _s2 ih => {
+      apply RedStar.step _ _; exact Syntax.ctor k A B' C
+      apply Red.ctor2 s1; apply ih
+    }
+  }
+
+
+  lemma red_ctor3 : C -β>* C' -> Syntax.ctor k A B C -β>* Syntax.ctor k A B C' := by {
+    intro step
+    induction step
+    case refl => apply RedStar.refl
+    case step C C' z s1 _s2 ih => {
+      apply RedStar.step _ _; exact Syntax.ctor k A B C'
+      apply Red.ctor3 s1; apply ih
+    }
+  }
+
+  lemma red_ctor :
+    A -β>* A' ->
+    B -β>* B' ->
+    C -β>* C' ->
+    Syntax.ctor k A B C -β>* Syntax.ctor k A' B' C'
+  := by {
+    intro s1 s2 s3
+    apply RedStar.trans _ _; exact Syntax.ctor k A' B C
+    apply red_ctor1 s1; apply RedStar.trans _ _; exact Syntax.ctor k A' B' C
+    apply red_ctor2 s2; apply red_ctor3 s3
+  }
+
+  lemma red_pi
+    : A -β>* A' -> x ∉ fv B ++ fv B' -> {_|-> x}B -β>* {_|-> x}B' -> pi m A B -β>* pi m A' B'
+  := by apply red_bind
+
+  lemma red_pi' {S : FvSet!}
+    : A -β>* A' -> ((x : Name) -> x ∉ S -> {_|-> x}B -β>* {_|-> x}B') -> pi m A B -β>* pi m A' B'
+  := by apply red_bind'
+
+  lemma red_lam
+    : A -β>* A' -> x ∉ fv B ++ fv B' -> {_|-> x}B -β>* {_|-> x}B' -> lam m A B -β>* lam m A' B'
+  := by apply red_bind
+
+  lemma red_lam' {S : FvSet!}
+    : A -β>* A' -> ((x : Name) -> x ∉ S -> {_|-> x}B -β>* {_|-> x}B') -> lam m A B -β>* lam m A' B'
+  := by apply red_bind'
+
+  lemma red_inter
+    : A -β>* A' -> x ∉ fv B ++ fv B' -> {_|-> x}B -β>* {_|-> x}B' -> pi m A B -β>* pi m A' B'
+  := by apply red_bind
+
+  lemma red_inter' {S : FvSet!}
+    : A -β>* A' -> ((x : Name) -> x ∉ S -> {_|-> x}B -β>* {_|-> x}B') -> inter A B -β>* inter A' B'
+  := by apply red_bind'
+
+  lemma red_app : f -β>* f' -> a -β>* a' -> app m f a -β>* app m f' a'
+  := by intro h1 h2; apply red_ctor h1 h2 RedStar.refl
+
+  lemma red_pair : t -β>* t' -> s -β>* s' -> a -β>* a' -> pair t s a -β>* pair t' s' a'
+  := by apply red_ctor
+
+  lemma red_fst : t -β>* t' -> fst t -β>* fst t'
+  := by intro h; apply red_ctor h RedStar.refl RedStar.refl
+
+  lemma red_snd : t -β>* t' -> snd t -β>* snd t'
+  := by intro h; apply red_ctor h RedStar.refl RedStar.refl
+
+  lemma red_eq : A -β>* A' -> a -β>* a' -> b -β>* b' -> eq A a b -β>* eq A' a' b'
+  := by apply red_ctor
+
+  lemma red_promote : t -β>* t' -> promote t -β>* promote t'
+  := by intro h; apply red_ctor h RedStar.refl RedStar.refl
+
+  lemma red_phi : a -β>* a' -> b -β>* b' -> e -β>* e' -> phi a b e -β>* phi a' b' e'
+  := by apply red_ctor
+
+  lemma red_norm : A -β>* A' -> (∀ z, ¬ A -β> z) -> A = A' := by {
+    intro step norm
+    induction step
+    case refl => simp
+    case step u u' v s1 _s2 _ih => {
+      exfalso; apply norm u' s1
+    }
+  }
+
+  lemma red_force_mode_pi_domain : Mode.pi_domain m K -β>* A -> A = Mode.pi_domain m K := by {
+    intro step
+    cases m <;> simp at * <;> cases step <;> simp [*]
+    case _ _ step _ => cases step
+    case _ _ step _ => cases step
+    case _ _ step _ => cases step
+  }
+
+  lemma red_force_mode_pi_codomain : Mode.pi_codomain m -β>* A -> A = Mode.pi_codomain m := by {
+    intro step
+    cases m <;> simp at * <;> cases step <;> simp [*]
+    case _ _ step _ => cases step
+    case _ _ step _ => cases step
+    case _ _ step _ => cases step 
+  }
+
+  lemma red_force_typeu : typeu -β>* A -> A = typeu := by {
+    intro step
+    cases step <;> simp [*]
+    case _ _ step _ => cases step
+  }
+
+  @[simp] lemma red_inv_pi_not_pi_domain : ¬ pi m1 A B -β>* Mode.pi_domain m2 K := by {
+    intro h
+    generalize lhsdef : pi m1 A B = lhs at *
+    generalize rhsdef : Mode.pi_domain m2 K = rhs at *
+    induction h generalizing m1 A B
+    case refl => {
+      subst lhsdef
+      cases m2 <;> simp at *
+    }
+    case step u u' z s1 s2 ih => {
+      subst lhsdef; cases s1 <;> simp at *
+      case bind1 A' step => apply @ih m1 A' B rfl rhsdef
+      case bind2 B' S step => apply @ih m1 A B' rfl rhsdef
+    }
+  }
+
+  @[simp] lemma red_inv_inter_not_pi_domain : ¬ inter A B -β>* Mode.pi_domain m K := by {
+    intro h
+    generalize lhsdef : inter A B = lhs at *
+    generalize rhsdef : Mode.pi_domain m K = rhs at *
+    induction h generalizing m A B
+    case refl => {
+      subst lhsdef
+      cases m <;> simp at *
+    }
+    case step u u' z s1 s2 ih => {
+      subst lhsdef; cases s1 <;> simp at *
+      case bind1 A' step => apply @ih A' B m rfl rhsdef
+      case bind2 B' S step => apply @ih A B' m rfl rhsdef
+    }
+  }
 
   -- lemma ctt_normal : ¬ (ctt -β> t) := sorry
   -- lemma cff_normal : ¬ (cff -β> t) := sorry
