Cedille/Theorem.lean
@@ -1,4 +1,3 @@
 
-import Cedille.Theorem.Preservation
 import Cedille.Theorem.ObjectConv1
 import Cedille.Theorem.ObjectConv2
