Cedille/Theorem/ObjectConv2.lean
@@ -4,16 +4,16 @@ import Cedille.Lemma
 
 namespace Cedille
 
-  lemma proof_red_to_object_red_step :
+  lemma proof_red_to_object_red_step (x : Name) :
     Γ ⊢ t : A ->
     t -β> s ->
-    (erase t) -β>* (erase s)
+    (erase x t) -β>* (erase x s)
   := sorry
 
-  lemma proof_red_to_object_red :
+  lemma proof_red_to_object_red (x : Name) :
     Γ ⊢ t : A ->
     t -β>* s ->
-    (erase t) -β>* (erase s)
+    (erase x t) -β>* (erase x s)
   := by {
     intros j step
     induction step
@@ -23,19 +23,18 @@ namespace Cedille
     }
   }
 
-  theorem proof_to_object_conv :
+  theorem proof_to_object_conv (x : Name) :
     Γ ⊢ t : A ->
     Γ ⊢ s : B ->
     t =β= s ->
-    (erase t) =β= (erase s)
+    (erase x t) =β= (erase x s)
   := by {
     intros j1 j2 e
     cases e
     case _ t1 t2 s1 e s2 =>
-    have s1 := proof_red_to_object_red j1 s1
-    have s2 := proof_red_to_object_red j2 s2
-    apply Conv.conv s1 s2 _
-    simp [*] -- idempotency of erasure
+    have s1 := proof_red_to_object_red x j1 s1
+    have s2 := proof_red_to_object_red x j2 s2
+    sorry
   }
 
 end Cedille
