Cedille/Theorem/Substitution.lean
@@ -4,7 +4,7 @@ import Cedille.Lemma
 
 namespace Cedille
 
-  theorem substitution {C : Term} :
+  theorem substitution {C : Term 0} :
     Γ1 ⊢ a : A ->
     (Γ1 ++ [x:A] ++ Γ2) ⊢ t : B ->
     (Γ1 ++ [x := a]Γ2) ⊢ [x := a]t : [x := a]A
