Common/Mathlib.lean
@@ -22,3 +22,6 @@ import Mathlib.Tactic.RenameBVar
 import Mathlib.Tactic.Replace
 
 import Mathlib.Data.Fin.Basic
+
+import Std.Data.Fin.Lemmas
+import Std.Data.List.Lemmas
