Common/Name.lean
@@ -1,4 +1,4 @@
-
+-- 
 import Common.Mathlib
 import Common.Util
 
@@ -19,9 +19,19 @@ instance : Ord Name where
     | Ordering.gt => Ordering.gt
 
 namespace Name
-  def beq_of_not_eq {a b : Name} : a ≠ b -> (a == b) = false := sorry
-  def not_eq_of_beq {a b : Name} : (a == b) = false -> a ≠ b := sorry
-  def beq_of_not_beq {a b : Name} : (a == b) ≠ true -> (a == b) = false := sorry 
+  def beq_of_not_eq {a b : Name} : a ≠ b -> (a == b) = false := by {
+    intro h
+    have lem : ¬ (a == b) = true := contra (@LawfulBEq.eq_of_beq Name _ _ a b) h
+    simp [*]
+  }
+
+  def not_eq_of_beq {a b : Name} : (a == b) = false -> a ≠ b := by {
+    intro h1 h2; subst h2
+    rw [LawfulBEq.rfl] at h1
+    contradiction
+  }
+
+  def beq_of_not_beq {a b : Name} : (a == b) ≠ true -> (a == b) = false := by simp [*] 
 
   def decEq (a : Name) (b : Name) : Decidable (a = b) :=
     match String.decEq a.1 b.1 with
@@ -61,13 +71,121 @@ namespace FvSet
 
   def not_mem_nil : x ∉ [] := by simp
 
-  def not_mem_left {A B : FvSet!} : x ∉ A ++ B -> x ∉ A := sorry
+  lemma not_mem_append {A B : FvSet!} : x ∉ A ++ B -> x ∉ A ∧ x ∉ B := by {
+    intro h
+    rewrite [List.mem_append_eq] at h
+    apply And.intro _ _
+    intro h2; apply h (Or.inl h2)
+    intro h2; apply h (Or.inr h2)
+  }
 
-  def not_mem_right {A B : FvSet!} : x ∉ A ++ B -> x ∉ B := sorry
+  def not_mem_left {A B : FvSet!} : x ∉ A ++ B -> x ∉ A := λ h => (not_mem_append h).1
+  def not_mem_right {A B : FvSet!} : x ∉ A ++ B -> x ∉ B := λ h => (not_mem_append h).2
 
-  def not_mem_head {A : FvSet!} : x ∉ y :: A -> x ≠ y := sorry
+  def not_mem_head {A : FvSet!} : x ∉ y :: A -> x ≠ y := List.ne_of_not_mem_cons
+  def not_mem_cons {A : FvSet!} : x ∉ y :: A -> x ∉ A := List.not_mem_of_not_mem_cons
 
-  def not_mem_cons {A : FvSet!} : x ∉ y :: A -> x ∉ A := sorry 
+  lemma subset_mem {x : Name} {A B : FvSet!} : A ⊆ B -> x ∈ A -> x ∈ B := by {
+    intro h1 h2
+    apply h1 h2
+  }
+
+  lemma subset_left {A B C : FvSet!} : A ⊆ B -> A ⊆ B ++ C := by {
+    intro h
+    induction A <;> simp at *
+    case cons hd tl ih => {
+      apply And.intro _ (ih h.2)
+      apply Or.inl h.1
+    }
+  }
+
+  lemma subset_right {A B C : FvSet!} : A ⊆ C -> A ⊆ B ++ C := by {
+    intro h
+    induction A <;> simp at *
+    case cons hd tl ih => {
+      apply And.intro _ (ih h.2)
+      apply Or.inr h.1
+    }
+  }
+
+  lemma subset_cons {A B : FvSet!} : x ∉ A -> A ⊆ x :: B -> A ⊆ B := by {
+    intro h1 h2
+    induction A <;> simp at *
+    case cons hd tl ih => {
+      replace h1 := demorgan h1
+      casesm* _ ∧ _; case _ e1 e2 e3 e4 =>
+      apply And.intro _ (ih e4 e2)
+      cases e1
+      case _ h => exfalso; subst h; contradiction
+      case _ h => exact h
+    }
+  }
+
+  lemma subset_trans {A B C : FvSet!} : A ⊆ B -> B ⊆ C -> A ⊆ C := by {
+    intro h1 h2
+    induction A generalizing B <;> simp at *
+    case cons hd tl ih => {
+      cases h1; case _ e1 e2 =>
+      apply And.intro (h2 e1) (ih e2 h2)
+    }
+  }
+
+  lemma subset_comm {A B C : FvSet!} : A ⊆ B ++ C -> A ⊆ C ++ B := by {
+    intro h
+    induction A generalizing B C <;> simp at *
+    case cons hd tl ih => {
+      apply And.intro _ (ih h.2)
+      cases h.1
+      case _ h => apply Or.inr h
+      case _ h => apply Or.inl h
+    }
+  }
+
+  lemma subset_append {A B C : FvSet!} : A ⊆ x :: (B ++ C) <-> A ⊆ (x :: B) ++ (x :: C) := by {
+    apply Iff.intro _ _
+    intro h
+    induction A generalizing B C <;> simp at *
+    case cons hd tl ih => {
+      apply And.intro _ (ih h.2)
+      cases h.1
+      case _ h => apply Or.inl h
+      case _ h => {
+        cases h
+        case _ h =>  apply Or.inr _; apply Or.inl h
+        case _ h => {
+          apply Or.inr _; apply Or.inr _; apply Or.inr h
+        }
+      }
+    }
+    intro h
+    induction A generalizing B C <;> simp at *
+    case cons hd tl ih => {
+      apply And.intro _ (ih h.2)
+      cases h.1
+      case _ h => apply Or.inl h
+      case _ h => {
+        cases h
+        case _ h => apply Or.inr _; apply Or.inl h
+        case _ h => {
+          cases h
+          case _ h => apply Or.inl h
+          case _ h => apply Or.inr _; apply Or.inr h
+        }
+      }
+    }
+  } 
+
+  lemma not_mem_subset_not_mem {A B : FvSet!} : x ∉ A -> B ⊆ A -> x ∉ B := by {
+    intro h1 h2
+    induction B generalizing A <;> simp at *
+    case cons hd tl ih => {
+      intro h
+      cases h
+      case _ h => subst h; apply h1 h2.1
+      case _ h => apply (ih h1 h2.2) h
+    }
+  }
+
 
 end FvSet
 
